\section{Bidirectional Type Checking for System-F}

\cite{Dunfield:2013}\cite{Jones:2007}

\subsection{Language}

Syntax:
\begin{align*}
  \begin{array}{lrcl}
    \text{Type Variables} &\alpha&\Coloneq &\cdots \\
    \text{Variables} &x&\Coloneq &\cdots \\
    \text{Mono Types}
    &\tau &\Coloneq &\alpha \\
    &&\mid &\tau_1 \to \tau_2 \\
    \text{Types}
    &\sigma &\Coloneq &\alpha \\
    &&\mid &\sigma_1 \to \sigma_2 \\
    &&\mid &\forall \alpha\ldotp \sigma \\
    \text{Terms}
    &e &\Coloneq &x \\
    &&\mid &\lambda x\ldotp e \\
    &&\mid &\lambda x: \sigma\ldotp e \\
    &&\mid &e_1\; e_2 \\
    &&\mid &e: \sigma \\
    \text{Contexts}
    &\Gamma &\Coloneq &\epsilon \\
    &&\mid &\Gamma_1 + \Gamma_2 \\
    &&\mid &x: \sigma \\
    &&\mid &\alpha
  \end{array}
\end{align*}

Context Member:
\begin{gather*}
  \infer{
    x: \sigma \in x:\sigma
  }{}
  \hspace{1em}
  \infer{
    x: \sigma \in \Gamma_1 + \Gamma_2
  }{
    x: \sigma \in \Gamma_1
  }
  \hspace{1em}
  \infer{
    x: \sigma \in \Gamma_1 + \Gamma_2
  }{
    x: \sigma \in \Gamma_2
  }
  \\
  \infer{
    \alpha \in \alpha
  }{}
  \hspace{1em}
  \infer{
    \alpha \in \Gamma_1 + \Gamma_2
  }{
    \alpha \in \Gamma_1
  }
  \hspace{1em}
  \infer{
    \alpha \in \Gamma_1 + \Gamma_2
  }{
    \alpha \in \Gamma_2
  }
\end{gather*}

Type Validity:
\begin{gather*}
  \infer{
    \Gamma \vdash \alpha
  }{
    \alpha \in \Gamma
  }
  \\
  \infer{
    \Gamma \vdash \sigma_1 \to \sigma_2
  }{
    \Gamma \vdash \sigma_1
    &
    \Gamma \vdash \sigma_2
  }
  \\
  \infer{
    \Gamma \vdash \forall \alpha\ldotp \sigma
  }{
    \Gamma, \alpha \vdash \sigma
  }
\end{gather*}

Term Typing (predicative):
\begin{gather*}
  \infer[\text{Var}]{
    \Gamma \vdash x: \sigma
  }{
    x:\sigma \in \Gamma
  }
  \\
  \infer[\text{Abs}]{
    \Gamma \vdash \lambda x\ldotp e: \sigma_1 \to \sigma_2
  }{
    \Gamma, x: \sigma_1\vdash e: \sigma_2
  }
  \\
  \infer[\text{AnnAbs}]{
    \Gamma \vdash \lambda x: \sigma_1\ldotp e: \sigma_1 \to \sigma_2
  }{
    \Gamma, x: \sigma_1\vdash e: \sigma_2
  }
  \\
  \infer[\text{App}]{
    \Gamma \vdash e_1\; e_2: \sigma
  }{
    \Gamma \vdash e_1: \sigma_2 \to \sigma
    &
    \Gamma \vdash e_2: \sigma_2
  }
  \\
  \infer[\text{Gen}]{
    \Gamma \vdash e: \forall \alpha\ldotp \sigma
  }{
    \Gamma, \alpha \vdash e: \sigma
  }
  \\
  \infer[\text{Inst}]{
    \Gamma \vdash e: \sigma[\alpha \assign \tau]
  }{
    \Gamma \vdash e: \forall \alpha\ldotp \sigma
    &
    \Gamma \vdash \tau
  }
\end{gather*}

\subsection{Bidirectional Typing}

Bidirectional Typing:
\begin{gather*}
  \infer[\text{Var}]{
    \Gamma \vdash x \Rightarrow \sigma
  }{
    x: \sigma \in \Gamma
  }
  \\
  \infer[\text{Extend}]{
    \Gamma \vdash e \Leftarrow \sigma_2
  }{
    \Gamma \vdash e \Rightarrow \sigma_1
    &
    \sigma_1 \leq \sigma_2
  }
  \\
  \infer[\text{Ann}]{
    \Gamma \vdash (e: \sigma) \Rightarrow \sigma
  }{
    \Gamma \vdash \sigma
    &
    \Gamma \vdash e \Leftarrow \sigma
  }
  \\
  \infer[\text{TyAbs}]{
    \Gamma \vdash e \Leftarrow \forall \alpha\ldotp \sigma
  }{
    \Gamma, \alpha \vdash e \Leftarrow \sigma
  }
  \\
  \infer[\text{TyApp}]{
    \Gamma \vdash \forall \alpha\ldotp \sigma_1 \Rightarrow e \Rightarrow \sigma_2
  }{
    \Gamma \vdash \tau
    &
    \Gamma \vdash \sigma_1[\alpha \assign \tau] \Rightarrow e \Rightarrow \sigma_2
  }
  \\
  \infer[\text{AbsI}]{
    \Gamma \vdash \lambda x\ldotp e \Leftarrow \sigma_1 \to \sigma_2
  }{
    \Gamma, x: \sigma_1 \vdash e \Leftarrow \sigma_2
  }
  \hspace{1em}
  \infer[\text{Abs}]{
    \Gamma \vdash \lambda x\ldotp e \Rightarrow \tau_1 \to \tau_2
  }{
    \Gamma \vdash \tau_1 \to \tau_2
    &
    \Gamma, x: \tau_1 \vdash e \Leftarrow \tau_2
  }
  \\
  \infer[\text{AnnAbsI}]{
    \Gamma \vdash \lambda x: \sigma_1\ldotp e \Leftarrow \sigma_1 \to \sigma_2
  }{
    \Gamma, x: \sigma_1 \vdash e \Leftarrow \sigma_2
  }
  \hspace{1em}
  \infer[\text{AnnAbs}]{
    \Gamma \vdash \lambda x: \sigma_1\ldotp e \Rightarrow \sigma_1 \to \tau_2
  }{
    \Gamma \vdash \sigma_1 \to \tau_2
    &
    \Gamma, x: \sigma_1 \vdash e \Leftarrow \tau_2
  }
  \\
  \infer[\text{AppI}]{
    \Gamma \vdash \sigma_1 \to \sigma_2 \Rightarrow e \Rightarrow \sigma_2
  }{
    \Gamma \vdash e \Leftarrow \sigma_1
  }
  \hspace{1em}
  \infer[\text{App}]{
    \Gamma \vdash e_1\; e_2 \Rightarrow \sigma
  }{
    \Gamma \vdash e_1 \Rightarrow \sigma_1
    &
    \Gamma \vdash \sigma_1 \Rightarrow e_2 \Rightarrow \sigma
  }
\end{gather*}

Subtyping:
\begin{gather*}
  \infer[\text{Var}]{
    \alpha \leq \alpha
  }{
    \alpha \in \Gamma
  }
  \\
  \infer[\text{Arrow}]{
    \Gamma \vdash \sigma_1 \to \sigma_2 \leq \sigma'_1 \to \sigma'_2
  }{
    \Gamma \vdash \sigma'_1 \leq \sigma_1
    &
    \Gamma \vdash \sigma_2 \leq \sigma'_2
  }
  \\
  \infer[\text{Spec}]{
    \Gamma \vdash \forall \alpha\ldotp \sigma_1 \leq \sigma_2
  }{
    \Gamma \vdash \tau
    &
    \Gamma \vdash \sigma_1[\alpha \assign \tau] \leq \sigma_2
  }
  \\
  \infer[\text{Skol}]{
    \Gamma \vdash \sigma_1 \leq \forall \alpha\ldotp \sigma_2
  }{
    \Gamma, \beta \vdash \sigma_1 \leq \sigma_2
  }
\end{gather*}

\subsection{Algorithmic Type Inference}

Algorithmic context:
\begin{align*}
  \begin{array}{rcl}
    \Gamma &\Coloneq &\epsilon \\
    &\mid &\Gamma, \alpha \\
    &\mid &\Gamma, x: \sigma \\
    &\mid &\Gamma, \hat{\alpha} \\
    &\mid &\Gamma, \hat{\alpha} = \tau \\
    &\mid &\Gamma, \alpha \mapsto \hat{\alpha}
  \end{array}
\end{align*}

Substitution:
\begin{gather*}
  \infer{[\Gamma]\alpha = \alpha}{}
  \\
  \infer{[\Gamma]\hat{\alpha} = \tau}{
    \hat{\alpha} = \tau \in \Gamma
  }
  \\
  \infer{[\Gamma](\sigma_1 \to \sigma_2) = \sigma_1' \to \sigma_2'}{
    [\Gamma](\sigma_1) = \sigma_1'
    &
    [\Gamma](\sigma_2) = \sigma_2'
  }
  \\
  \infer{[\Gamma](\forall \alpha\ldotp \sigma) = \forall \alpha\ldotp \sigma'}{
    [\Gamma]\sigma = \sigma'
  }
\end{gather*}

Bidirectional typing:
\begin{gather*}
  \infer[\text{Sub}]{\Gamma \vdash e \Leftarrow \sigma_2 \mid \Delta}{
    \Gamma \vdash e \Rightarrow \sigma_1 \mid \Theta
    &
    \Theta \vdash [\Theta]\sigma_1 \leq [\Theta]\sigma_2 \mid \Delta
  }
  \\
  \infer[\text{Var}]{\Gamma \vdash x \Rightarrow \sigma \mid \Gamma}{
    x: \sigma \in \Gamma
  }
  \\
  \infer[\text{Ann}]{\Gamma \vdash e: \sigma \Rightarrow \sigma \mid \Delta}{
    \Gamma \vdash \sigma
    &
    \Gamma \vdash e \Leftarrow \sigma \mid \Delta
  }
  \\
  \infer[\text{TyAbs}]{\Gamma \vdash e \Leftarrow \forall \alpha\ldotp \sigma \mid \Delta}{
    \Gamma,\alpha \vdash e \Leftarrow \sigma \mid \Delta, \alpha, \Theta
  }
  \\
  \infer[\text{TyApp}]{\Gamma \vdash \forall \alpha\ldotp \sigma_1 \Rightarrow e \Rightarrow \sigma_2 \mid \Delta}{
    \Gamma,\hat{\alpha} \vdash \sigma_1[\alpha \assign \hat{\alpha}] \Rightarrow e \Rightarrow \sigma_2 \mid \Delta
  }
  \\
  \infer[\text{AbsI}]{\Gamma \vdash \lambda x\ldotp e \Leftarrow \sigma_1 \to \sigma_2 \mid \Delta}{
    \Gamma, x: \sigma_1 \vdash e \Leftarrow \sigma_2 \mid \Delta, x: \sigma_1, \Theta
  }
  \\
  \infer[\text{Abs}]{\Gamma \vdash \lambda x\ldotp e \Rightarrow \hat{\alpha_1} \to \hat{\alpha_2} \mid \Delta}{
    \Gamma, \hat{\alpha_1}, \hat{\alpha_2}, x: \hat{\alpha_1} \vdash e \Leftarrow \hat{\alpha_2} \mid \Delta, x: \hat{\alpha_1}, \Theta
  }
  \\
  \infer[\text{AppU}]{\Gamma_1, \hat{\alpha_1}, \Gamma_2 \vdash \hat{\alpha_1} \Rightarrow e \Rightarrow \hat{\alpha_3} \mid \Delta}{
    \Gamma_1, \hat{\alpha_3}, \hat{\alpha_2}, \hat{\alpha_1} = \hat{\alpha_2} \to \hat{\alpha_3} \vdash e \Leftarrow \hat{\alpha_2} \mid \Delta
  }
  \\
  \infer[\text{AppI}]{\Gamma \vdash \sigma_1 \to \sigma_2 \Rightarrow e \Rightarrow \sigma_2 \mid \Delta}{
    \Gamma \vdash e \Leftarrow \sigma_1 \mid \Delta
  }
  \\
  \infer[\text{App}]{\Gamma \vdash e_1\; e_2 \Rightarrow \sigma_2 \mid \Delta}{
    \Gamma \vdash e_1 \Rightarrow \sigma_1 \mid \Theta
    &
    \Theta \vdash [\Theta]\sigma_1 \Rightarrow e_2 \Rightarrow \sigma_2 \mid \Delta
  }
\end{gather*}

Subtyping:
\begin{gather*}
  \infer{\Gamma \vdash \alpha \leq \alpha \mid \Gamma}{
    \alpha \in \Gamma
  }
  \\
  \infer{\Gamma \vdash \hat{\alpha} \leq \hat{\alpha} \mid \Gamma}{
    \hat{\alpha} \in \Gamma
  }
  \\
  \infer{\Gamma \vdash \sigma_1 \to \sigma_2 \leq \sigma_1' \to \sigma_2' \mid \Delta}{
    \Gamma \vdash \sigma_1 \leq \sigma_1' \mid \Theta
    &
    \Theta \vdash [\Theta]\sigma_2 \leq [\Theta]\sigma_2' \mid \Delta
  }
  \\
  \infer{\Gamma \vdash \forall \alpha\ldotp \sigma_1 \leq \sigma_2 \mid \Delta}{
    \Gamma, \alpha \mapsto \hat{\alpha}, \hat{\alpha} \vdash \sigma_1[\alpha \assign \hat{\alpha}] \leq \sigma_2 \mid \Delta, \alpha \mapsto \hat{\alpha}, \Theta
  }
  \\
  \infer{\Gamma \vdash \sigma_1 \leq \forall \alpha\ldotp \sigma_2 \mid \Delta}{
    \Gamma, \alpha \vdash \sigma_1 \leq \sigma_2 \mid \Delta, \alpha, \Theta
  }
  \\
  \infer{\Gamma \vdash \hat{\alpha_1} \leq \sigma_2 \mid \Delta}{
    \hat{\alpha_1} \not\in \mathit{ftv}(\sigma_2)
    &
    \hat{\alpha_1} \in \Gamma
    &
    \Gamma \vdash \hat{\alpha_1} \simeq \sigma_2 \mid \Delta
  }
  \\
  \infer{\Gamma \vdash \sigma_1 \leq \hat{\alpha_2} \mid \Delta}{
    \hat{\alpha_2} \not\in \mathit{ftv}(\sigma_1)
    &
    \hat{\alpha_2} \in \Gamma
    &
    \Gamma \vdash \sigma_1 \simeq \hat{\alpha_2} \mid \Delta
  }
\end{gather*}

Instantiation:
\begin{gather*}
  \infer{\Gamma_1, \hat{\alpha}, \Gamma_2 \vdash \hat{\alpha} \simeq \tau \mid \Gamma_1, \hat{\alpha} = \tau, \Gamma_2}{
    \Gamma_1 \vdash \tau
  }
  \\
  \infer{\Gamma_1, \hat{\alpha}, \Gamma_2 \vdash \tau \simeq \hat{\alpha} \mid \Gamma_1, \hat{\alpha} = \tau, \Gamma_2}{
    \Gamma_1 \vdash \tau
  }
  \\
  \infer{\Gamma_1, \hat{\alpha_1}, \Gamma_2, \hat{\alpha_2}, \Gamma_3 \vdash \hat{\alpha_1} \simeq \hat{\alpha_2} \mid \Gamma_1, \hat{\alpha_1}, \Gamma_2, \hat{\alpha_2} = \hat{\alpha_1}, \Gamma_3}{}
  \\
  \infer{\Gamma_1, \hat{\alpha_1}, \Gamma_2 \vdash \hat{\alpha_1} \simeq \sigma_2 \to \sigma_3 \mid \Delta}{
    \Gamma_1, \hat{\alpha_3}, \hat{\alpha_2}, \hat{\alpha_1} = \hat{\alpha_2} \to \hat{\alpha_3}, \Gamma_2 \vdash \sigma_2 \simeq \hat{\alpha_2} \mid \Theta
    &
    \Theta \vdash \hat{\alpha_3} \simeq [\Theta]\sigma_3 \mid \Delta
  }
  \\
  \infer{\Gamma_1, \hat{\alpha_1}, \Gamma_2 \vdash \sigma_2 \to \sigma_3 \simeq \hat{\alpha_1} \mid \Delta}{
    \Gamma_1, \hat{\alpha_3}, \hat{\alpha_2}, \hat{\alpha_1} = \hat{\alpha_2} \to \hat{\alpha_3}, \Gamma_2 \vdash \hat{\alpha_2} \simeq \sigma_2 \mid \Theta
    &
    \Theta \vdash [\Theta]\sigma_3 \simeq \hat{\alpha_3} \mid \Delta
  }
  \\
  \infer{\Gamma_1, \hat{\alpha_1}, \Gamma_2 \vdash \hat{\alpha_1} \simeq \forall \alpha_2\ldotp \sigma_2 \mid \Delta}{
    \Gamma_1, \hat{\alpha_1}, \Gamma_2, \alpha_2 \vdash \hat{\alpha_1} \simeq \sigma_2 \mid \Delta, \alpha_2, \Theta
  }
  \\
  \infer{\Gamma_1, \hat{\alpha_2}, \Gamma_2 \vdash \forall \alpha_1\ldotp \sigma_1 \simeq \hat{\alpha_2} \mid \Delta}{
    \Gamma_1, \hat{\alpha_2}, \Gamma_2, \alpha_1 \mapsto \hat{\alpha_1}, \hat{\alpha_1} \vdash \sigma_1[\alpha_1 \assign \hat{\alpha_1}] \simeq \hat{\alpha_2} \mid \Delta, \alpha_1 \mapsto \hat{\alpha_1}, \Theta
  }
\end{gather*}
