\section{Hindley/Milner Type System}

\cite{Lee:1998}

\subsection{Language}

$X = \{x,y,z,\ldots\}$，$\mathcal{A} = \{\alpha, \beta, \ldots\}$

$E$
\begin{align*}
  \begin{array}{rcll}
    e
    & \Coloneq & \text{\texttt{()}} \\
    & \mid & x \\
    & \mid & \lambda x\ldotp e \\
    & \mid & e\; e \\
    & \mid & \mathbf{let}\;x = e\;\mathbf{in}\;e \\
    & \mid & \mathbf{fix}\;f\;\lambda x\ldotp e
  \end{array}
\end{align*}

$T$
\begin{align*}
  \begin{array}{rcll}
    \tau
    & \Coloneq & \mathbf{unit} \\
    & \mid & \alpha \\
    & \mid & \tau \to \tau
  \end{array}
\end{align*}

$\Sigma$
\begin{align*}
  \begin{array}{rcll}
    \sigma
    & \Coloneq & \forall \vec{\alpha}\ldotp \sigma
  \end{array}
\end{align*}

$\Gamma = \mathcal{A} \xrightarrow{\mathrm{fin}} \Sigma$

\subsection{Type System}

\begin{align*}
  \forall \vec{\alpha}\ldotp \tau_1 \succ \tau_2 &\iff \exists S\ldotp S(\tau_1) = \tau_2 \land \mathrm{dom}(S) \\
  \mathrm{Gen}(\Gamma, \tau) &= \forall \vec{\alpha}\ldotp \tau &(\vec{\alpha} = \mathit{ftv}(\tau) \backslash \mathit{ftv}(\Gamma))
\end{align*}

\begin{gather*}
  \infer{\Gamma \vdash \text{\texttt{()}}: \mathbf{unit}}{}
  \\
  \infer{\Gamma \vdash x: \tau}{
    \Gamma(x) \succ \tau
  }
  \\
  \infer{\Gamma \vdash \lambda x\ldotp e: \tau_1 \to \tau_2}{
    \Gamma + x:\tau_1\vdash e: \tau_2
  }
  \\
  \infer{\Gamma \vdash e_1\; e_2: \tau}{
    \Gamma \vdash e_1: \tau_2 \to \tau
    &
    \Gamma \vdash e_2: \tau_2
  }
  \\
  \infer{\Gamma \vdash \mathbf{let}\; x = e_1\; \mathbf{in}\; e_2: \tau}{
    \Gamma \vdash e_1: \tau_1
    &
    \Gamma + x: \mathrm{Gen}(\Gamma, \tau_1) \vdash e_2: \tau
  }
  \\
  \infer{\Gamma \vdash \mathbf{fix}\;f\;\lambda x\ldotp e: \tau}{
    \Gamma + f: \tau \vdash \lambda x\ldotp e: \tau
  }
\end{gather*}

TODO: 停止するかが怪しいのでチェック．\cite{Grabmuller:2006}にはこの定義で書いてある
\begin{gather*}
  \infer{\mathcal{U}(\alpha, \alpha) = \emptyset}{}
  \\
  \infer{\mathcal{U}(\alpha_1, \alpha_2) = \{\alpha_1 \mapsto \beta, \alpha_2 \mapsto \beta\}}{
    \alpha_1 \neq \alpha_2
    &
    \text{fresh $\beta$}
  }
  \\
  \infer{\mathcal{U}(\mathbf{unit}, \mathbf{unit}) = \emptyset}{}
  \\
  \infer{\mathcal{U}(\alpha, \mathbf{unit}) = \{\alpha \mapsto \mathbf{unit}\}}{}
  \\
  \infer{\mathcal{U}(\mathbf{unit}, \alpha) = \{\alpha \mapsto \mathbf{unit}\}}{}
  \\
  \infer{\mathcal{U}(\alpha, \tau_1 \to \tau_2) = \{\alpha \mapsto \tau_1 \to \tau_2\}}{}
  \\
  \infer{\mathcal{U}(\tau_1 \to \tau_2, \alpha) = \{\alpha \mapsto \tau_1 \to \tau_2\}}{}
  \\
  \infer{\mathcal{U}(\tau_1 \to \tau_2, \tau'_1 \to \tau'_2) = S_2S_1}{
    \mathcal{U}(\tau_1, \tau'_1) = S_1
    &
    \mathcal{U}(S_1(\tau_2), S_1(\tau'_2)) = S_2
  }
\end{gather*}

\begin{theorem}
  $\mathcal{U}(\tau_1, \tau_2) = S$ ならば，$S(\tau_1) = S(\tau_2)$．
\end{theorem}

\section{Algorithm W}

\begin{theorem}
  以下は同値
  \begin{itemize}
    \item $\mathcal{U}(\tau_1, \tau_2) = S$ を満たす $S$ が存在する．
    \item $S(\tau_1) = S(\tau_2)$ を満たす $S$ が存在する．
  \end{itemize}
\end{theorem}

\begin{gather*}
  \infer{\mathcal{W}(\Gamma, \text{\texttt{()}}) = (\emptyset, \mathbf{unit})}{}
  \\
  \infer{\mathcal{W}(\Gamma, x) = (\emptyset, [\vec{\alpha} \assign \vec{\beta}]\tau)}{
    \Gamma(x) = \forall\vec{\alpha}\ldotp \tau
    &
    \text{fresh $\vec{\beta}$}
  }
  \\
  \infer{\mathcal{W}(\Gamma, \lambda x\ldotp e) = (S_1, S_1(\beta) \to \tau_1)}{
    \text{fresh $\beta$}
    &
    \mathcal{W}(\Gamma + x:\beta, e) = (S_1, \tau_1)
  }
  \\
  \infer{\mathcal{W}(\Gamma, e_1\; e_2) = (S_3S_2S_1, S_3(\beta))}{
    \mathcal{W}(\Gamma, e_1) = (S_1, \tau_1)
    &
    \mathcal{W}(S_1(\Gamma), e_2) = (S_2, \tau_2)
    &
    \text{fresh $\beta$}
    &
    \mathcal{U}(S_2(\tau), \tau_2 \to \beta) = S_3
  }
  \\
  \infer{\mathcal{W}(\Gamma, \mathbf{let}\;x = e_1\;\mathbf{in}\;e_2) = (S_2S_1, \tau_2)}{
    \mathcal{W}(\Gamma, e_1) = (S_1, \tau_1)
    &
    \Gamma_1 = S_1(\Gamma)
    &
    \mathcal{W}(\Gamma_1 + x:\mathrm{Gen}(\Gamma_1, \tau_1), e_2) = (S_2, \tau_2)
  }
  \\
  \infer{\mathcal{W}(\Gamma, \mathbf{fix}\;f\;\lambda x\ldotp e) = (S_2S_1, S_2(\tau_1))}{
    \text{fresh $\beta$}
    &
    \mathcal{W}(\Gamma + f:\beta, \lambda x\ldotp e) = (S_1, \tau_1)
    &
    \mathcal{U}(S_1(\beta), \tau_1) = S_2
  }
\end{gather*}

\begin{theorem}
  以下は同値
  \begin{itemize}
    \item $\mathcal{W}(\Gamma_0, e) = (S, \tau_0)$，$S(\Gamma_0) = \Gamma$，$S(\tau_0) = \tau$ を満たす $S$，$\Gamma_0$，$\tau_0$ が存在する．
    \item $\Gamma \vdash e: \tau$．
  \end{itemize}
\end{theorem}

\section{Algorithm M}

\begin{gather*}
  \infer{\mathcal{M}(\Gamma, \text{\texttt{()}}, \rho) = S}{
    \mathcal{U}(\rho, \mathbf{unit}) = S
  }
  \\
  \infer{\mathcal{M}(\Gamma, x, \rho) = S}{
    \mathcal{U}(\rho, [\vec{\beta} \assign \vec{\alpha}]\tau) = S
    &
    \Gamma(x) = \forall \vec{\alpha}\ldotp \tau
    &
    \text{fresh $\vec{\beta}$}
  }
  \\
  \infer{\mathcal{M}(\Gamma, \lambda x\ldotp e, \rho) = S_2S_1}{
    \mathcal{U}(\rho, \beta_1 \to \beta_2) = S_1
    &
    \text{fresh $\beta_1, \beta_2$}
    &
    \mathcal{M}(S_1(\Gamma) + x:S_1(\beta_1), e, S_1(\beta_2)) = S_2
  }
  \\
  \infer{\mathcal{M}(\Gamma, e_1\;e_2, \rho) = S_2S_1}{
    \mathcal{M}(\Gamma, e_1, \beta \to \rho) = S_1
    &
    \text{fresh $\beta$}
    &
    \mathcal{M}(S_1(\Gamma), e_2, S_1(\beta)) = S_2
  }
  \\
  \infer{\mathcal{M}(\Gamma, \mathbf{let}\;x = e_1\;\mathbf{in}\;e_2, \rho) = S_2S_1}{
    \mathcal{M}(\Gamma, e_1, \beta) = S_1
    &
    \text{fresh $\beta$}
    &
    \mathcal{M}(S_1(\Gamma) + x:\mathrm{Gen}(\Gamma, S_1(\beta)), e_2, S_1(\rho)) = S_2
  }
  \\
  \infer{\mathcal{M}(\Gamma, \mathbf{fix}\;f\;\lambda x\ldotp e, \rho) = S}{
    \mathcal{M}(\Gamma + f:\rho, \lambda x\ldotp e, \rho) = S
  }
\end{gather*}

\begin{theorem}
  以下は同値
  \begin{itemize}
    \item $\mathcal{M}(\Gamma_0, e, \rho) = S$，$S(\Gamma_0) = \Gamma$，$S(\rho) = \tau$ を満たす $S$，$\Gamma_0$，$\rho$ が存在する．
    \item $\Gamma \vdash e: \tau$．
  \end{itemize}
\end{theorem}
