\section{λμ-Calculus}

Alias: λμ \cite{Selinger:2001}\cite{Rocheteau:2005}

\subsection{Syntax}

\begin{align*}
  \begin{array}{rclr}
  \tau
  & \Coloneq & t &(\text{type variable}) \\
  & \mid & \top &(\text{top type}) \\
  & \mid & \tau \multi \tau &(\text{product type}) \\
  & \mid & \tau \to \tau &(\text{function type}) \\
  & \mid & \bot &(\text{bottom type}) \\
  e
  & \Coloneq & x &(\text{variable}) \\
  & \mid & \langle\rangle &(\text{top value}) \\
  & \mid & \langle e, e\rangle &(\text{product}) \\
  & \mid & \pi_1 e &(\text{left projection}) \\
  & \mid & \pi_2 e &(\text{right projection}) \\
  & \mid & \lambda x: \tau\ldotp e &(\text{abstraction}) \\
  & \mid & e\; e &(\text{application}) \\
  & \mid & [\alpha] e &(\text{naming}) \\
  & \mid & \mu \alpha: \tau\ldotp e &(\text{un-naming}) \\
  \Gamma
  & \Coloneq & \cdot \\
  & \mid & \Gamma, x: \tau \\
  \Delta
  & \Coloneq & \cdot \\
  & \mid & \alpha: \tau, \Delta
  \end{array}
\end{align*}

Environment Reference:

$\fbox{$\Gamma(x) = \tau$}$

\begin{gather*}
  \infer{(\Gamma, x': \tau)(x) = \tau}{
    x = x'
  }
  \hspace{2em}
  \infer{(\Gamma, x': \tau')(x) = \tau}{
    x \neq x'
    &
    \Gamma(x) = \tau
  }
\end{gather*}

$\fbox{$\Delta(\alpha) = \tau$}$

\begin{gather*}
  \infer{(\alpha': \tau, \Delta)(\alpha) = \tau}{
    \alpha = \alpha'
  }
  \hspace{2em}
  \infer{(\alpha': \tau', \Delta)(\alpha) = \tau}{
    \alpha \neq \alpha'
    &
    \Delta(\alpha) = \tau
  }
\end{gather*}

\subsection{Typing Semantics}

$\fbox{$\Gamma \vdash e: \tau \mid \Delta$}$

\begin{gather*}
  \infer[\text{T-Var}]{\Gamma \vdash x: \tau \mid \Delta}{
    \Gamma(x) = \tau
  }
  \\
  \infer[\text{T-Top}]{\Gamma \vdash \langle\rangle: \top \mid \Delta}{}
  \\
  \infer[\text{T-Product}]{\Gamma \vdash \langle e_1, e_2\rangle: \tau_1 \times \tau_2 \mid \Delta}{
    \Gamma \vdash e_1: \tau_1 \mid \Delta
    &
    \Gamma \vdash e_2: \tau_2 \mid \Delta
  }
  \\
  \infer[\text{T-Proj-1}]{\Gamma \vdash \pi_1 e: \tau_1 \mid \Delta}{
    \Gamma \vdash e: \tau_1 \times \tau_2 \mid \Delta
  }
  \\
  \infer[\text{T-Proj-2}]{\Gamma \vdash \pi_2 e: \tau_2 \mid \Delta}{
    \Gamma \vdash e: \tau_1 \times \tau_2 \mid \Delta
  }
  \\
  \infer[\text{T-Abs}]{\Gamma \vdash \lambda x: \tau_1\ldotp e: \tau_1 \to \tau_2 \mid \Delta}{
    \Gamma, x: \tau_1 \vdash e: \tau_2 \mid \Delta
  }
  \\
  \infer[\text{T-App}]{\Gamma \vdash e_1\; e_2: \tau \mid \Delta}{
    \Gamma \vdash e_1: \tau_2 \to \tau \mid \Delta
    &
    \Gamma \vdash e_2: \tau_2 \mid \Delta
  }
  \\
  \infer[\text{T-Name}]{\Gamma \vdash [\alpha] e: \bot \mid \Delta}{
    \Delta(\alpha) = \tau
    &
    \Gamma \vdash e: \tau \mid \Delta
  }
  \\
  \infer[\text{T-Unname}]{\Gamma \vdash (\mu \alpha: \tau\ldotp e): \tau \mid \Delta}{
    \Gamma \vdash e: \bot \mid \alpha: \tau, \Delta
  }
\end{gather*}

\subsection{Equivalence}

$\fbox{$\Gamma \vdash e_1 \equiv e_2: \tau \mid \Delta$}$

\begin{gather*}
  \infer[\text{Eq-$\beta$-Lam}]{\Gamma \vdash (\lambda x: \tau_2\ldotp e_1)\; e_2 \equiv e_1[x \assign e_2]: \tau \mid \Delta}{
    \Gamma, x: \tau_2 \vdash e_1: \tau \mid \Delta
    &
    \Gamma \vdash e_2: \tau_2 \mid \Delta
  }
  \\
  \infer[\text{Eq-$\eta$-Lam}]{\Gamma \vdash (\lambda x: \tau_1\ldotp e\; x) \equiv e: \tau_1 \to \tau_2 \mid \Delta}{
    x \not\in \freevar(e)
    &
    \Gamma \vdash e: \tau_1 \to \tau_2 \mid \Delta
  }
  \\
  \infer[\text{Eq-$\eta$-Top}]{\Gamma \vdash \langle\rangle \equiv e: \top \mid \Delta}{
    \Gamma \vdash e: \top \mid \Delta
  }
  \\
  \infer[\text{Eq-$\beta$-Product-1}]{\Gamma \vdash \pi_1\langle e_1, e_2\rangle \equiv e_1: \tau_1 \mid \Delta}{
    \Gamma \vdash e_1: \tau_1 \mid \Delta
    &
    \Gamma \vdash e_2: \tau_2 \mid \Delta
  }
  \\
  \infer[\text{Eq-$\beta$-Product-2}]{\Gamma \vdash \pi_2\langle e_1, e_2\rangle \equiv e_2: \tau_2 \mid \Delta}{
    \Gamma \vdash e_1: \tau_1 \mid \Delta
    &
    \Gamma \vdash e_2: \tau_2 \mid \Delta
  }
  \\
  \infer[\text{Eq-$\eta$-Product}]{\Gamma \vdash \langle \pi_1 e, \pi_2 e\rangle \equiv e: \tau_1 \multi \tau_2 \mid \Delta}{
    \Gamma \vdash e: \tau_1 \multi \tau_2 \mid \Delta
  }
  \\
  \infer[\text{Eq-$\zeta$-Product-1}]{\Gamma \vdash \pi_1 (\mu \alpha: \tau_1 \multi \tau_2\ldotp e) \equiv \mu \alpha_1: \tau_1\ldotp e[[\alpha](-) \assign [\alpha_1](\pi_1 (-))]: \tau_1 \mid \Delta}{
    \alpha_1 \not\in \freevar(e)
    &
    \Gamma \vdash e: \bot \mid \alpha: \tau_1 \multi \tau_2, \Delta
  }
  \\
  \infer[\text{Eq-$\zeta$-Product-2}]{\Gamma \vdash \pi_2 (\mu \alpha: \tau_1 \multi \tau_2\ldotp e) \equiv \mu \alpha_2: \tau_2\ldotp e[[\alpha](-) \assign [\alpha_2](\pi_2 (-))]: \tau_2 \mid \Delta}{
    \alpha_2 \not\in \freevar(e)
    &
    \Gamma \vdash e: \bot \mid \alpha: \tau_1 \multi \tau_2, \Delta
  }
  \\
  \infer[\text{Eq-$\beta$-Mu}]{\Gamma \vdash [\alpha_1](\mu \alpha_2: \tau_\alpha\ldotp e) \equiv e[\alpha_2 \assign \alpha_1]: \bot \mid \Delta}{
    \Gamma \vdash e: \bot \mid \alpha_2: \tau_\alpha, \Delta
  }
  \\
  \infer[\text{Eq-$\eta$-Mu}]{\Gamma \vdash (\mu \alpha: \tau\ldotp [\alpha]e) \equiv e: \tau \mid \Delta}{
    \Gamma \vdash e: \tau \mid \Delta
  }
  \\
  \infer[\text{Eq-$\zeta$-Mu}]{\Gamma \vdash (\mu \alpha: \tau_1 \to \tau_2\ldotp e_1)\; e_2 \equiv \mu \alpha_2: \tau_2\ldotp e_1[[\alpha](-) \assign [\alpha_2]((-)\; e_2)]: \tau_2 \mid \Delta}{
    \alpha_2 \not\in \freevar(e_1) \cup \freevar(e_2)
    &
    \Gamma \vdash e_1: \bot \mid \alpha: \tau_1 \to \tau_2, \Delta
    &
    \Gamma \vdash e_2: \tau_2 \mid \Delta
  }
\end{gather*}

\subsection{Elaboration (Call-By-Value)}

$\fbox{$\Gamma \vdash e: \tau \elaborate e'$}$

\begin{gather*}
  \infer{\Gamma \vdash x_0: \tau \elaborate \lambda x_k: K_\tau\ldotp x_k\; x_{x_0}}{
    \Gamma(x_{x_0}) = V_\tau
  }
  \\
  \infer{\Gamma \vdash \langle\rangle: \top \elaborate \lambda x_k: K_\top\ldotp x_k\; \langle\rangle}{}
  \\
  \infer{\Gamma \vdash \langle e_1, e_2\rangle: \tau_1 \multi \tau_2 \elaborate \lambda x_k: K_{\tau_1 \multi \tau_2}\ldotp e_1'\; (\lambda x_1: V_{\tau_1}\ldotp e_2'\; (\lambda x_2: V_{\tau_2}\ldotp x_k\; \langle x_1, x_2\rangle))}{
    \Gamma \vdash e_1: \tau_1 \elaborate e_1'
    &
    \Gamma \vdash e_2: \tau_2 \elaborate e_2'
  }
  \\
  \infer{\Gamma \vdash \pi_1 e: \tau_1 \elaborate \lambda x_k: K_{\tau_1}\ldotp e'\; (\lambda x: V_{\tau_1} \multi V_{\tau_2}\ldotp x_k\; (\pi_1 x))}{
    \Gamma \vdash e: \tau_1 \multi \tau_2 \elaborate e'
  }
  \\
  \infer{\Gamma \vdash \pi_2 e: \tau_2 \elaborate \lambda x_k: K_{\tau_2}\ldotp e'\; (\lambda x: V_{\tau_1} \multi V_{\tau_2}\ldotp x_k\; (\pi_2 x))}{
    \Gamma \vdash e: \tau_1 \multi \tau_2 \elaborate e'
  }
  \\
  \infer{\Gamma \vdash (\lambda x_0: \tau_1\ldotp e): \tau_1 \to \tau_2 \elaborate \lambda x_k: K_{\tau_1 \to \tau_2}\ldotp x_k\; (\lambda x: V_{\tau_1} \multi K_{\tau_2}\ldotp (\lambda x_{x_0}: V_{\tau_1}\ldotp e')\; (\pi_1 x)\; (\pi_2 x))}{
    \Gamma, x_{x_0}: V_{\tau_1} \vdash e: \tau_2 \elaborate e'
  }
  \\
  \infer{\Gamma \vdash e_1\; e_2: \tau \elaborate \lambda x_k: K_{\tau}\ldotp e_1'\; (\lambda x_1: V_{\tau_2 \to \tau}\ldotp e_2'\; (\lambda x_2: V_{\tau_2}\ldotp x_1\; \langle x_2, x_k\rangle))}{
    \Gamma \vdash e_1: \tau_2 \to \tau \elaborate e_1'
    &
    \Gamma \vdash e_2: \tau_2 \elaborate e_2'
  }
  \\
  \infer{\Gamma \vdash (\mu \alpha: \tau\ldotp e): \tau \elaborate \lambda x_\alpha: K_\tau\ldotp e'\; (\lambda x: \bot\ldotp \symcase x\; \{\})}{
    \Gamma, x_\alpha: K_\tau \vdash e: \bot \elaborate e'
  }
  \\
  \infer{\Gamma \vdash [\alpha] e: \tau \elaborate \lambda x_k: K_\bot\ldotp e'\; x_\alpha}{
    \Gamma(x_\alpha) = K_\tau
    &
    \Gamma \vdash e: \tau \elaborate e'
  }
\end{gather*}

$\fbox{$V_\tau = \tau'$}$

\begin{gather*}
  \infer{V_\top = \top}{}
  \\
  \infer{V_{\tau_1 \multi \tau_2} = V_{\tau_1'} \multi V_{\tau_2'}}{
    V_{\tau_1} = \tau_1'
    &
    V_{\tau_2} = \tau_2'
  }
  \\
  \infer{V_{\tau_1 \to \tau_2} = \tau_1' \multi \tau_2' \to R}{
    V_{\tau_1} = \tau_1'
    &
    K_{\tau_2} = \tau_2'
  }
  \\
  \infer{V_\bot = \bot}{}
\end{gather*}

Abbreviation:

\begin{align*}
  K_\tau &\defrel{=} V_\tau \to R \\
  C_\tau &\defrel{=} K_\tau \to R
\end{align*}

\begin{theorem}
  $\Gamma \vdash e: \tau \elaborate e'$ ならば，$\Gamma \vdash e': C_\tau$．
\end{theorem}

\begin{theorem}
  $\Gamma \vdash e: \tau \mid \Delta \iff V(\Gamma), K(\Delta) \vdash e: \tau \elaborate e'$．ただし，
  \begin{align*}
    V(\Gamma) &\defrel{=} \left\{\begin{array}{ll}
      V(\Gamma'), x_{x'}: V_{\tau'} &(\Gamma = \Gamma', x': \tau') \\
      \cdot &(\Gamma = \cdot)
    \end{array}\right. \\
    K(\Delta) &\defrel{=} \left\{\begin{array}{ll}
      x_\alpha: K_\tau, K(\Delta') &(\Delta = \alpha: \tau, \Delta') \\
      \cdot &(\Delta = \cdot)
    \end{array}\right. \text{．}
  \end{align*}
\end{theorem}

\subsection{Elaboration (Call-By-Name)}

$\fbox{$\Gamma \vdash e: \tau \elaborate e'$}$

\begin{gather*}
  \infer{\Gamma \vdash x_0: \tau \elaborate \lambda x_k: K_\tau\ldotp x_{x_0}\; x_k}{
    \Gamma(x_{x_0}) = C_\tau
  }
  \\
  \infer{\Gamma \vdash \langle\rangle: \top \elaborate \lambda x_k: \bot\ldotp \symcase x_k\; \{\}}{}
  \\
  \infer{\Gamma \vdash \langle e_1, e_2\rangle: \tau_1 \multi \tau_2 \elaborate \lambda x_k: K_{\tau_1} \plus K_{\tau_2}\ldotp \symcase x_k\; \{x_{k_1}\ldotp e_1'\; x_{k_1} \mid x_{k_2}\ldotp e_2'\; x_{k_2}\}}{
    \Gamma \vdash e_1: \tau_1 \elaborate e_1'
    &
    \Gamma \vdash e_2: \tau_2 \elaborate e_2'
  }
  \\
  \infer{\Gamma \vdash \pi_1 e: \tau_1 \elaborate \lambda x_k: K_{\tau_1}\ldotp e'\; (i_1 x_k)}{
    \Gamma \vdash e: \tau_1 \multi \tau_2 \elaborate e'
  }
  \\
  \infer{\Gamma \vdash (\lambda x_1: \tau_1\ldotp e): \tau_1 \to \tau_2 \elaborate \lambda x_k: C_{\tau_1} \multi K_{\tau_2}\ldotp e'[x_{x_1} \assign \pi_1 x_k]\; (\pi_2 x_k)}{
    \Gamma, x_{x_1}: C_{\tau_1} \vdash e: \tau_2 \elaborate e'
  }
  \\
  \infer{\Gamma \vdash e_1\; e_2: \tau \elaborate \lambda x_k: K_\tau\ldotp e_1'\; \langle e_2', x_k\rangle}{
    \Gamma \vdash e_1: \tau_2 \to \tau \elaborate e_1'
    &
    \Gamma \vdash e_2: \tau_2 \elaborate e_2'
  }
  \\
  \infer{\Gamma \vdash [\alpha] e: \bot \elaborate \lambda x_k: K_\bot\ldotp e'\; x_\alpha}{
    \Gamma(x_\alpha) = K_\tau
    &
    \Gamma \vdash e: \tau \elaborate e'
  }
  \\
  \infer{\Gamma \vdash (\mu \alpha: \tau\ldotp e): \tau \elaborate \lambda x_\alpha: K_\tau\ldotp e'\; \langle\rangle}{
    \Gamma, x_\alpha: K_\tau \vdash e: \bot \elaborate e'
  }
\end{gather*}

$\fbox{$K_\tau = \tau'$}$

\begin{gather*}
  \infer{K_\top = \bot}{}
  \\
  \infer{K_{\tau_1 \multi \tau_2} = \tau_1' \plus \tau_2'}{
    K_{\tau_1} = \tau_1'
    &
    K_{\tau_2} = \tau_2'
  }
  \\
  \infer{K_{\tau_1 \to \tau_2} = \tau_1' \multi \tau_2'}{
    C_{\tau_1} = \tau_1'
    &
    K_{\tau_2} = \tau_2'
  }
  \\
  \infer{K_\bot = \top}{}
\end{gather*}

Abbreviation:

\begin{align*}
  C_\tau &\defrel{=} K_\tau \to R
\end{align*}

\begin{theorem}
  $\Gamma \vdash e: \tau \elaborate e'$ ならば，$\Gamma \vdash e': C_\tau$．
\end{theorem}

\begin{theorem}
  $\Gamma \vdash e: \tau \mid \Delta \iff C(\Gamma), K(\Delta) \vdash e: \tau \elaborate e'$．ただし，
  \begin{align*}
    C(\Gamma) &\defrel{=} \left\{\begin{array}{ll}
      C(\Gamma'), x_{x'}: C_{\tau'} &(\Gamma = \Gamma', x': \tau') \\
      \cdot &(\Gamma = \cdot)
    \end{array}\right. \\
    K(\Delta) &\defrel{=} \left\{\begin{array}{ll}
      x_\alpha: K_\tau, K(\Delta') &(\Delta = \alpha: \tau, \Delta') \\
      \cdot &(\Delta = \cdot)
    \end{array}\right. \text{．}
  \end{align*}
\end{theorem}
