\section{Simply Typed λ-Calculus}

Alias: STLC，$\lambda^{\to}$ \cite{Girard:1989}

\subsection{Syntax}

\begin{align*}
  e
  &\BNFassign x &(\text{variable}) \\
  &\BNFor e\; e &(\text{application}) \\
  &\BNFor \lambda x: \tau\ldotp e &(\text{abstraction}) \\
  &\BNFor c_A &(\text{constant}) \\
  \tau
  &\BNFassign A &(\text{atomic type}) \\
  &\BNFor \tau \to \tau &(\text{function type}) \\
  \Gamma
  &\BNFassign \cdot &(\text{empty}) \\
  &\BNFor \Gamma, x: \tau &(\text{cons})
\end{align*}

Convention:

\begin{align*}
  \tau_1 \to \tau_2 \to \cdots \to \tau_n &\defrel{=} \tau_1 \to (\tau_2 \to (\cdots \to \tau_n) \cdots ) \\
  e_1\; e_2\; \cdots \; e_n &\defrel{=} (\cdots(e_1\; e_2)\cdots)\; e_n)
\end{align*}

Environment Reference:

$\fbox{$\Gamma(x) = \tau$}$

\begin{gather*}
  \infer{(\Gamma, x': \tau)(x) = \tau}{
    x = x'
  }
  \hspace{2em}
  \infer{(\Gamma, x': \tau)(x) = \tau}{
    x \neq x'
    &
    \Gamma(x) = \tau
  }
\end{gather*}

Free Variable:

$\fbox{$\freevar(e) = \{\overline{x'}\}$}$

\begin{gather*}
  \infer{\freevar(x) = \{x\}}{}
  \hspace{2em}
  \infer{\freevar(e_1\; e_2) = X_1 \cup X_2}{
    \freevar(e_1) = X_1
    &
    \freevar(e_2) = X_2
  }
  \hspace{2em}
  \infer{\freevar(\lambda x: \tau\ldotp e) = X \rcomplement \{x\}}{
    \freevar(e) = X
  }
  \hspace{2em}
  \infer{\freevar(c_A) = \emptyset}{}
\end{gather*}

Substitution:

部分関数 $\{x_1 \mapsto e_1, \ldots, x_n \mapsto e_n\}$ を，$[x_1 \assign e_1, \ldots, x_n \assign e_n]$ または $[x_1, \ldots, x_n \assign e_1, \ldots, e_n]$ と表記する．

$\fbox{$e[\overline{x' \assign e'}] = e''$}$

\begin{gather*}
\infer{x[\overline{x'} \assign \overline{e'}] = e}{
  [\overline{x'} \assign \overline{e'}](x) = e
}
\hspace{2em}
\infer{x[\overline{x'} \assign \overline{e'}]= x}{
  x \not\in \dom([\overline{x'} \assign \overline{e'}])
}
\\
\infer{(e_1\; e_2)[\overline{x'} \assign \overline{e'}] = e''_1\; e''_2}{
  e_1[\overline{x'} \assign \overline{e'}] = e''_1
  &
  e_2[\overline{x'} \assign \overline{e'}] = e''_2
}
\hspace{2em}
\infer{(\lambda x: \tau\ldotp e)[\overline{x'} \assign \overline{e'}] = \lambda x: \tau\ldotp e''}{
  e([\overline{x'} \assign \overline{e'}]\restrict_{\dom([\overline{x'} \assign \overline{e'}]) \rcomplement \{x\}}) = e''
}
\hspace{2em}
\infer{c_A[\overline{x'} \assign \overline{e'}] = c_A}{}
\end{gather*}

$\alpha$-Equality:

$\fbox{$e_1 \equiv_\alpha e_2$}$

\begin{gather*}
  \infer{x_1 \equiv_\alpha x_2}{
    x_1 = x_2
  }
  \hspace{2em}
  \infer{\lambda x_1: \tau\ldotp e_1 \equiv_\alpha \lambda x_2: \tau\ldotp e_2}{
    x' \not\in \freevar(e_1) \cup \freevar(e_2)
    &
    e_1[x_1 \assign x'] \equiv_\alpha e_2[x_2 \assign x']
  }
  \hspace{2em}
  \infer{e_1\; e'_1 \equiv_\alpha e_2\; e'_2}{
    e_1 \equiv_\alpha e_2
    &
    e'_1 \equiv_\alpha e'_2
  }
  \hspace{2em}
  \infer{c_A \equiv_\alpha c_A}{}
\end{gather*}

\begin{theorem}[Correctness of Substitution]
  式 $e$，置換 $[\overline{x'} \assign \overline{e'}]$ について，$X = \dom([\overline{x'} \assign \overline{e'}])$ とした時，
  \begin{align*}
    \freevar(e[\overline{x'} \assign \overline{e'}]) = (\freevar(e) \rcomplement X) \cup \bigcup_{x \in \freevar(e) \cap X} \freevar([\overline{x'} \assign \overline{e'}](x))\text{．}
  \end{align*}
\end{theorem}

\begin{theorem}[$\alpha$-Equality Does Not Touch Free Variables]
  $e_1 \equiv_\alpha e_2$ ならば，$\freevar(e_1) = \freevar(e_2)$．
\end{theorem}

\subsection{Typing Semantics}

$\fbox{$\Gamma \vdash e: \tau$}$

\begin{gather*}
  \infer[\text{T-Var}]{\Gamma \vdash x: \tau}{\Gamma(x) = \tau}
  \\
  \infer[\text{T-Abs}]{\Gamma \vdash \lambda x: \tau_1\ldotp e: \tau_1 \to \tau_2}{
    \Gamma, x: \tau_1 \vdash e: \tau_2
  }
  \\
  \infer[\text{T-App}]{\Gamma \vdash e_1\; e_2: \tau}{
    \Gamma \vdash e_1: \tau_2 \to \tau
    &
    \Gamma \vdash e_2: \tau_2
  }
  \\
  \infer[\text{T-Const}]{\Gamma \vdash c_A: A}{}
\end{gather*}

特に，$\cdot \vdash e: \tau$ の時，$e: \tau$ と表記．

\subsection{Evaluation Semantics (Call-By-Value)}

\begin{align*}
  v
  &\BNFassign \lambda x: \tau\ldotp e \\
  &\BNFor c_A \\
  C
  &\BNFassign [] \\
  &\BNFor C\; e \\
  &\BNFor v\; C
\end{align*}

Small Step:

$\fbox{$e \smalleval e'$}$

\begin{gather*}
  \infer{(\lambda x: \tau\ldotp e)\; v \smalleval e[x \assign v]}{}
  \\
  \infer{C[e] \smalleval C[e']}{
    e \smalleval e'
  }
\end{gather*}

Big Step:

$\fbox{$e \bigeval v$}$

\begin{gather*}
  \infer{e_1\; e_2 \bigeval v}{
    e_1 \bigeval \lambda x:\tau\ldotp e'_1
    &
    e_2 \bigeval v_2
    &
    e'_1[x \assign v_2] \bigeval v
  }
\end{gather*}

\begin{theorem}[Adequacy of Small Step and Big Step]
  $e \smalleval^* v \textiff e \bigeval v$．
\end{theorem}

\begin{theorem}[Type Soundness]
  $e: \tau$ の時，$e \smalleval^* v$，$e \bigeval v$ となる $v = \normalform(\smalleval, e)$ が存在し，
  \begin{itemize}
    \item $\tau = \tau_1 \to \tau_2$ の時，$v \equiv_\alpha \lambda x':\tau_1\ldotp e'$ となる $\lambda x':\tau'\ldotp e'$ が存在する．
    \item $\tau = A$ の時，$v \equiv_\alpha c_A$ となる $c_A$ が存在する．
  \end{itemize}
\end{theorem}

\subsection{Equational Reasoning}

$\fbox{$\Gamma \vdash e_1 \equiv e_2: \tau$}$

\begin{gather*}
  \infer[\text{Eq-$\beta$-Lam}]{\Gamma \vdash (\lambda x: \tau\ldotp e_1)\; e_2 \equiv e_1[x \assign e_2]: \tau}{
    \Gamma, x: \tau \vdash e_1: \tau_2 \to \tau
    &
    \Gamma \vdash e_2: \tau_2
  }
  \hspace{2em}
  \infer[\text{Eq-$\eta$-Lam}]{\Gamma \vdash (\lambda x: \tau_1\ldotp e\; x) \equiv e: \tau_1 \to \tau_2}{
    x \not\in \freevar(e)
    &
    \Gamma \vdash e: \tau_1 \to \tau_2
  }
  \\
  \infer[\text{Eq-$\alpha$-Refl}]{\Gamma \vdash e_1 \equiv e_2: \tau}{
    e_1 \equiv_\alpha e_2
    &
    \Gamma \vdash e_1: \tau
    &
    \Gamma \vdash e_2: \tau
  }
  \\
  \infer[\text{Eq-Sym}]{\Gamma \vdash e_1 \equiv e_2: \tau}{
    \Gamma \vdash e_2 \equiv e_1: \tau
  }
  \hspace{2em}
  \infer[\text{Eq-Trans}]{\Gamma \vdash e_1 \equiv e_3: \tau}{
    \Gamma \vdash e_1 \equiv e_2: \tau
    &
    \Gamma \vdash e_2 \equiv e_3: \tau
  }
  \\
  \infer[\text{Eq-Cong-Abs}]{\Gamma \vdash \lambda x: \tau\ldotp e_1 \equiv \lambda x: \tau\ldotp e_2: \tau \to \tau'}{
    \Gamma, x: \tau \vdash e_1 \equiv e_2: \tau'
  }
  \hspace{2em}
  \infer[\text{Eq-Cong-App}]{\Gamma \vdash e_1\; e'_1 \equiv e_2\; e'_2: \tau}{
    \Gamma \vdash e_1 \equiv e_2: \tau' \to \tau
    &
    \Gamma \vdash e'_1 \equiv e'_2: \tau'
  }
\end{gather*}

特に，$\cdot \vdash e_1 \equiv e_2: \tau$ の時，$e_1 \equiv e_2: \tau$ と表記．

\begin{theorem}[Respect Typing]
  $\Gamma \vdash e_1 \equiv e_2: \tau$ ならば，$\Gamma \vdash e_1: \tau$ かつ $\Gamma \vdash e_2: \tau$．
\end{theorem}

\begin{theorem}[Respect Evaluation]
  \theolabel{stlc:smallstep-equiv}
  $e_1 \equiv e_2: \tau$ の時，$e'_1 \smalleval^* e_1$，$e_2 \smalleval^* e'_2$ ならば $e'_1 \equiv e'_2: \tau$．
\end{theorem}

\begin{corollary}
  $e_1 \equiv e_2: \tau$ の時，$e_1 \smalleval^* e'_1$，$e_2 \smalleval^* e'_2$ ならば $e'_1 \equiv e'_2: \tau$．
\end{corollary}
\begin{proof}
  $e_1 \smalleval^* e_1$ より，\theoref{stlc:smallstep-equiv}から $e_1 \equiv e'_2: \tau$．よって，T-Sym から $e'_2 \equiv e_1: \tau$ であり，$e'_2 \smalleval^* e'_2$ より\theoref{stlc:smallstep-equiv}から $e'_2 \equiv e'_1: \tau$．故に，T-Sym から $e'_1 \equiv e'_2: \tau$．
\end{proof}
